New sequential machine

src/sequential/Debt.v
@@ -16,6 +16,7 @@ Require Import Event.
 Set Implicit Arguments.
 
 
+
 Definition get_machine_event (e: ProgramEvent.t): MachineEvent.t :=
   match e with
   | ProgramEvent.syscall e => MachineEvent.syscall e
@@ -23,70 +24,61 @@ Definition get_machine_event (e: ProgramEvent.t): MachineEvent.t :=
   | _ => MachineEvent.silent
   end.
 
-Definition is_atomic_event (e: ProgramEvent.t): Prop :=
+Definition is_atomic_event (e: ProgramEvent.t): bool :=
   match e with
-  | ProgramEvent.silent | ProgramEvent.failure => False
-  | ProgramEvent.syscall _ | ProgramEvent.fence _ _ => True
+  | ProgramEvent.silent | ProgramEvent.failure => false
+  | ProgramEvent.syscall _ | ProgramEvent.fence _ _ => true
   | ProgramEvent.read _ _ ord => Ordering.le Ordering.plain ord
   | ProgramEvent.write _ _ ord => Ordering.le Ordering.plain ord
   | ProgramEvent.update _ _ _ ordr ordw =>
-    Ordering.le Ordering.plain ordr /\ Ordering.le Ordering.plain ordw
+    Ordering.le Ordering.plain ordr && Ordering.le Ordering.plain ordw
   end.
 
 Definition is_accessing (e: ProgramEvent.t): option Loc.t :=
   match e with
   | ProgramEvent.silent | ProgramEvent.failure | ProgramEvent.syscall _ | ProgramEvent.fence _ _ => None
-  | ProgramEvent.read loc _ _ | ProgramEvent.write loc _ _ | ProgramEvent.update loc _ _ _ _ => Some loc
+  | ProgramEvent.read l _ _ | ProgramEvent.write l _ _ | ProgramEvent.update l _ _ _ _ => Some l
   end.
 
-Definition is_release_event (e: ProgramEvent.t): Prop :=
+Definition is_release (e: ProgramEvent.t): bool :=
   match e with
-  | ProgramEvent.syscall _ => True
-  | ProgramEvent.silent | ProgramEvent.failure | ProgramEvent.read _ _ _ => False
+  | ProgramEvent.syscall _ => true
+  | ProgramEvent.silent | ProgramEvent.failure | ProgramEvent.read _ _ _ => false
   | ProgramEvent.fence _ ord | ProgramEvent.write _ _ ord | ProgramEvent.update _ _ _ _ ord => Ordering.le Ordering.strong_relaxed ord
   end.
 
-Definition is_acquire_event (e: ProgramEvent.t): Prop :=
+Definition is_acquire (e: ProgramEvent.t): bool :=
   match e with
-  | ProgramEvent.syscall _ => True
-  | ProgramEvent.silent | ProgramEvent.failure | ProgramEvent.write _ _ _ => False
+  | ProgramEvent.syscall _ => true
+  | ProgramEvent.silent | ProgramEvent.failure | ProgramEvent.write _ _ _ => false
   | ProgramEvent.read _ _ ord | ProgramEvent.update _ _ _ ord _ => Ordering.le Ordering.acqrel ord
-  | ProgramEvent.fence ordr ordw => ordw = Ordering.seqcst  \/ Ordering.le Ordering.acqrel ordr
+  | ProgramEvent.fence ordr ordw => Ordering.le Ordering.seqcst ordw || Ordering.le Ordering.acqrel ordr
   end.
 
 
 Module Perm.
   Variant t: Type :=
-  | none
-  | full
+  | low
+  | high
   .
+
+  Definition meet (p0 p1: t): t :=
+    match p0, p1 with
+    | high, high => high
+    | _, _ => low
+    end.
+
+  Definition join (p0 p1: t): t :=
+    match p0, p1 with
+    | low, low => low
+    | _, _ => high
+    end.
 
   Definition le (p0 p1: t): bool :=
     match p0, p1 with
-    | none, _ => true
-    | _, full => true
+    | low, _ => true
+    | _, high => true
     | _, _ => false
-    end.
-End Perm.
-
-Module Perms.
-  Definition t := Loc.t -> Perm.t.
-End Perms.
-
-Module Flag.
-  Variant t :=
-  | written
-  | unwritten
-  | debt
-  .
-
-  Definition le (f_tgt f_src: t): bool :=
-    match f_tgt, f_src with
-    | debt, _ => true
-    | _, debt => false
-    | unwritten, _ => true
-    | _, unwritten => false
-    | _, written => true
     end.
 
   Program Instance le_PreOrder: PreOrder le.
@@ -98,13 +90,306 @@ Module Flag.
   Proof.
     ii. destruct x, y, z; ss.
   Qed.
+
+  Lemma meet_le_l p0 p1:
+    le (meet p0 p1) p0.
+  Proof.
+    destruct p0, p1; ss.
+  Qed.
+
+  Lemma meet_le_r p0 p1:
+    le (meet p0 p1) p1.
+  Proof.
+    destruct p0, p1; ss.
+  Qed.
+
+  Lemma meet_spec p0 p1 p
+        (LE0: le p p0)
+        (LE1: le p p1)
+    :
+      le p (meet p0 p1).
+  Proof.
+    destruct p, p0, p1; ss.
+  Qed.
+
+  Lemma meet_mon_l p0 p1 p
+        (LE: le p0 p1)
+    :
+      le (meet p0 p) (meet p1 p).
+  Proof.
+    destruct p, p0, p1; ss.
+  Qed.
+
+  Lemma meet_mon_r p0 p1 p
+        (LE: le p0 p1)
+    :
+      le (meet p p0) (meet p p1).
+  Proof.
+    destruct p, p0, p1; ss.
+  Qed.
+
+  Lemma join_ge_l p0 p1:
+    le p0 (join p0 p1).
+  Proof.
+    destruct p0, p1; ss.
+  Qed.
+
+  Lemma join_ge_r p0 p1:
+    le p1 (join p0 p1).
+  Proof.
+    destruct p0, p1; ss.
+  Qed.
+
+  Lemma join_spec p0 p1 p
+        (LE0: le p0 p)
+        (LE1: le p1 p)
+    :
+      le (join p0 p1) p.
+  Proof.
+    destruct p, p0, p1; ss.
+  Qed.
+
+  Lemma join_mon_l p0 p1 p
+        (LE: le p0 p1)
+    :
+      le (join p0 p) (join p1 p).
+  Proof.
+    destruct p, p0, p1; ss.
+  Qed.
+
+  Lemma join_mon_r p0 p1 p
+        (LE: le p0 p1)
+    :
+      le (join p p0) (join p p1).
+  Proof.
+    destruct p, p0, p1; ss.
+  Qed.
+End Perm.
+
+
+Module Perms.
+  Definition t := Loc.t -> Perm.t.
+
+  Definition meet (p0 p1: t): t :=
+    fun loc => Perm.meet (p0 loc) (p1 loc).
+
+  Definition join (p0 p1: t): t :=
+    fun loc => Perm.join (p0 loc) (p1 loc).
+
+  Definition update (loc: Loc.t) (p: Perm.t) (ps: t): t :=
+    fun loc' => if Loc.eq_dec loc loc' then p else ps loc'.
+
+  Definition acquired (p: t) (p_acq: t): Loc.t -> bool :=
+    fun loc => Perm.le (p_acq loc) (p loc).
+
+  Definition le (p0 p1: t): Prop :=
+    forall loc, Perm.le (p0 loc) (p1 loc).
+
+  Program Instance le_PreOrder: PreOrder le.
+  Next Obligation.
+  Proof.
+    ii. refl.
+  Qed.
+  Next Obligation.
+  Proof.
+    ii. etrans; eauto.
+  Qed.
+
+  Lemma meet_le_l p0 p1:
+    le (meet p0 p1) p0.
+  Proof.
+    ii. eapply Perm.meet_le_l; eauto.
+  Qed.
+
+  Lemma meet_le_r p0 p1:
+    le (meet p0 p1) p1.
+  Proof.
+    ii. eapply Perm.meet_le_r; eauto.
+  Qed.
+
+  Lemma meet_spec p0 p1 p
+        (LE0: le p p0)
+        (LE1: le p p1)
+    :
+      le p (meet p0 p1).
+  Proof.
+    ii. eapply Perm.meet_spec; eauto.
+  Qed.
+
+  Lemma meet_mon_l p0 p1 p
+        (LE: le p0 p1)
+    :
+      le (meet p0 p) (meet p1 p).
+  Proof.
+    ii. eapply Perm.meet_mon_l; eauto.
+  Qed.
+
+  Lemma meet_mon_r p0 p1 p
+        (LE: le p0 p1)
+    :
+      le (meet p p0) (meet p p1).
+  Proof.
+    ii. eapply Perm.meet_mon_r; eauto.
+  Qed.
+
+  Lemma join_ge_l p0 p1:
+    le p0 (join p0 p1).
+  Proof.
+    ii. eapply Perm.join_ge_l; eauto.
+  Qed.
+
+  Lemma join_ge_r p0 p1:
+    le p1 (join p0 p1).
+  Proof.
+    ii. eapply Perm.join_ge_r; eauto.
+  Qed.
+
+  Lemma join_spec p0 p1 p
+        (LE0: le p0 p)
+        (LE1: le p1 p)
+    :
+      le (join p0 p1) p.
+  Proof.
+    ii. eapply Perm.join_spec; eauto.
+  Qed.
+
+  Lemma join_mon_l p0 p1 p
+        (LE: le p0 p1)
+    :
+      le (join p0 p) (join p1 p).
+  Proof.
+    ii. eapply Perm.join_mon_l; eauto.
+  Qed.
+
+  Lemma join_mon_r p0 p1 p
+        (LE: le p0 p1)
+    :
+      le (join p p0) (join p p1).
+  Proof.
+    ii. eapply Perm.join_mon_r; eauto.
+  Qed.
+End Perms.
+
+
+Module Flag.
+  Definition t := bool.
+
+  Definition meet (f0 f1: t): t := andb f0 f1.
+
+  Definition join (f0 f1: t): t := orb f0 f1.
+
+  Definition le (f0 f1: t): bool := implb f0 f1.
+
+  Program Instance le_PreOrder: PreOrder le.
+  Next Obligation.
+  Proof.
+    ii. destruct x; ss.
+  Qed.
+  Next Obligation.
+  Proof.
+    ii. destruct x, y, z; ss.
+  Qed.
+
+  Lemma meet_le_l f0 f1:
+    le (meet f0 f1) f0.
+  Proof.
+    destruct f0, f1; ss.
+  Qed.
+
+  Lemma meet_le_r f0 f1:
+    le (meet f0 f1) f1.
+  Proof.
+    destruct f0, f1; ss.
+  Qed.
+
+  Lemma meet_spec f0 f1 f
+        (LE0: le f f0)
+        (LE1: le f f1)
+    :
+      le f (meet f0 f1).
+  Proof.
+    destruct f, f0, f1; ss.
+  Qed.
+
+  Lemma meet_mon_l f0 f1 f
+        (LE: le f0 f1)
+    :
+      le (meet f0 f) (meet f1 f).
+  Proof.
+    destruct f, f0, f1; ss.
+  Qed.
+
+  Lemma meet_mon_r f0 f1 f
+        (LE: le f0 f1)
+    :
+      le (meet f f0) (meet f f1).
+  Proof.
+    destruct f, f0, f1; ss.
+  Qed.
+
+  Lemma join_ge_l f0 f1:
+    le f0 (join f0 f1).
+  Proof.
+    destruct f0, f1; ss.
+  Qed.
+
+  Lemma join_ge_r f0 f1:
+    le f1 (join f0 f1).
+  Proof.
+    destruct f0, f1; ss.
+  Qed.
+
+  Lemma join_spec f0 f1 f
+        (LE0: le f0 f)
+        (LE1: le f1 f)
+    :
+      le (join f0 f1) f.
+  Proof.
+    destruct f, f0, f1; ss.
+  Qed.
+
+  Lemma join_mon_l f0 f1 f
+        (LE: le f0 f1)
+    :
+      le (join f0 f) (join f1 f).
+  Proof.
+    destruct f, f0, f1; ss.
+  Qed.
+
+  Lemma join_mon_r f0 f1 f
+        (LE: le f0 f1)
+    :
+      le (join f f0) (join f f1).
+  Proof.
+    destruct f, f0, f1; ss.
+  Qed.
 End Flag.
+
 
 Module Flags.
   Definition t := Loc.t -> Flag.t.
 
-  Definition le (f_tgt f_src: t): Prop :=
-    forall loc, Flag.le (f_tgt loc) (f_src loc).
+  Definition empty: t := fun _ => false.
+
+  Definition is_empty (f: t): Prop := forall loc, f loc = false.
+
+  Definition update (loc: Loc.t) (f: Flag.t) (fs: t): t :=
+    fun loc' => if Loc.eq_dec loc' loc then f else (fs loc').
+
+  Definition add (loc: Loc.t) (f: t): t :=
+    fun loc' => if Loc.eq_dec loc' loc then true else (f loc').
+
+  Definition sub (loc: Loc.t) (f: t): t :=
+    fun loc' => if Loc.eq_dec loc' loc then false else (f loc').
+
+  Definition meet (f0 f1: t): t :=
+    fun loc => Flag.meet (f0 loc) (f1 loc).
+
+  Definition join (f0 f1: t): t :=
+    fun loc => Flag.join (f0 loc) (f1 loc).
+
+  Definition le (f0 f1: t): Prop :=
+    forall loc, Flag.le (f0 loc) (f1 loc).
 
   Program Instance le_PreOrder: PreOrder le.
   Next Obligation.
@@ -114,93 +399,100 @@ Module Flags.
   Next Obligation.
   Proof.
     ii. etrans; eauto.
+  Qed.
+
+  Lemma meet_le_l f0 f1:
+    le (meet f0 f1) f0.
+  Proof.
+    ii. eapply Flag.meet_le_l; eauto.
+  Qed.
+
+  Lemma meet_le_r f0 f1:
+    le (meet f0 f1) f1.
+  Proof.
+    ii. eapply Flag.meet_le_r; eauto.
+  Qed.
+
+  Lemma meet_spec f0 f1 f
+        (LE0: le f f0)
+        (LE1: le f f1)
+    :
+      le f (meet f0 f1).
+  Proof.
+    ii. eapply Flag.meet_spec; eauto.
+  Qed.
+
+  Lemma meet_mon_l f0 f1 f
+        (LE: le f0 f1)
+    :
+      le (meet f0 f) (meet f1 f).
+  Proof.
+    ii. eapply Flag.meet_mon_l; eauto.
+  Qed.
+
+  Lemma meet_mon_r f0 f1 f
+        (LE: le f0 f1)
+    :
+      le (meet f f0) (meet f f1).
+  Proof.
+    ii. eapply Flag.meet_mon_r; eauto.
+  Qed.
+
+  Lemma join_ge_l f0 f1:
+    le f0 (join f0 f1).
+  Proof.
+    ii. eapply Flag.join_ge_l; eauto.
+  Qed.
+
+  Lemma join_ge_r f0 f1:
+    le f1 (join f0 f1).
+  Proof.
+    ii. eapply Flag.join_ge_r; eauto.
+  Qed.
+
+  Lemma join_spec f0 f1 f
+        (LE0: le f0 f)
+        (LE1: le f1 f)
+    :
+      le (join f0 f1) f.
+  Proof.
+    ii. eapply Flag.join_spec; eauto.
+  Qed.
+
+  Lemma join_mon_l f0 f1 f
+        (LE: le f0 f1)
+    :
+      le (join f0 f) (join f1 f).
+  Proof.
+    ii. eapply Flag.join_mon_l; eauto.
+  Qed.
+
+  Lemma join_mon_r f0 f1 f
+        (LE: le f0 f1)
+    :
+      le (join f f0) (join f f1).
+  Proof.
+    ii. eapply Flag.join_mon_r; eauto.
   Qed.
 End Flags.
 
-Module SeqCell.
-   Definition t := (Const.t * Flag.t)%type.
 
-   Definition flag (c: t): Flag.t := snd c.
+Module ValueMap.
+  Definition t := Loc.t -> Const.t.
 
-   Definition debt (c: t): t :=
-     let (v, f) := c in (v, Flag.debt).
+  Definition write (loc: Loc.t) (v: Const.t) (vs: t): t :=
+    fun loc' => if Loc.eq_dec loc' loc then v else (vs loc').
 
-   Definition write (v: Const.t): t :=
-     (v, Flag.written).
+  Definition read (loc: Loc.t) (vs: t) := vs loc.
 
-   Definition update (v1: Const.t) (c: t): t :=
-     let (v0, f) := c in (v1, f).
+  Definition acquire (cond: Loc.t -> bool) (vs_acq: t) (vs: t): t :=
+    fun loc => if (cond loc) then (vs loc) else (vs_acq loc).
 
-   (* checked at final *)
-   Definition le (c0 c1: t): Prop :=
-     match c0, c1 with
-     | (v0, f0), (v1, f1) => v0 = v1 /\ Flag.le f0 f1
-     end.
+  Definition release (vs: t) (d: Flags.t): t :=
+    fun loc => if (d loc) then Const.undef else (vs loc).
 
-   (* checked every moment *)
-   Definition le_partial (c0 c1: t): Prop :=
-     Flag.le (flag c0) (flag c1).
-
-   Program Instance le_PreOrder: PreOrder le.
-   Next Obligation.
-   Proof.
-     ii. destruct x; ss. split; auto. refl.
-   Qed.
-   Next Obligation.
-   Proof.
-     ii. destruct x, y, z; ss.
-     des. subst. splits; auto. etrans; eauto.
-   Qed.
-
-   Program Instance le_partial_PreOrder: PreOrder le_partial.
-   Next Obligation.
-   Proof.
-     ii. unfold le_partial in *. refl.
-   Qed.
-   Next Obligation.
-   Proof.
-     ii. unfold le_partial in *. etrans; eauto.
-   Qed.
-
-   Lemma le_le_partial c0 c1 (LE: le c0 c1)
-     :
-       le_partial c0 c1.
-   Proof.
-     destruct c0, c1. ss. des; auto.
-   Qed.
-
-   Definition init (v: Const.t): t := (v, Flag.unwritten).
-
-   Variant release: forall (c_before c_released c_after: t), Prop :=
-   | release_normal
-       c0 c1
-       (LE: le c0 c1)
-     :
-       release c1 c0 c0
-   | release_debt
-       c0 c1
-     :
-       release c0 c1 (debt c0)
-   .
-End SeqCell.
-
-
-Module SeqMemory.
-  Definition t := Loc.t -> SeqCell.t.
-
-  Definition flags (m: t): Flags.t := fun loc => snd (m loc).
-
-  Definition update (loc: Loc.t) (c: SeqCell.t) (m: t): t :=
-    fun loc' => if Loc.eq_dec loc' loc then c else (m loc').
-
-  Definition write (loc: Loc.t) (val: Const.t) (m: t): t :=
-    update loc (SeqCell.write val) m.
-
-  Definition le (m_tgt m_src: t): Prop :=
-    forall loc, SeqCell.le (m_tgt loc) (m_src loc).
-
-  Definition le_partial (m_tgt m_src: t): Prop :=
-    Flags.le (flags m_tgt) (flags m_src).
+  Definition le (vs0 vs1: t): Prop :=
+    forall loc, Const.le (vs0 loc) (vs1 loc).
 
   Program Instance le_PreOrder: PreOrder le.
   Next Obligation.
@@ -211,40 +503,190 @@ Module SeqMemory.
   Proof.
     ii. etrans; eauto.
   Qed.
-
-  Program Instance le_partial_PreOrder: PreOrder le_partial.
-  Next Obligation.
-  Proof.
-    ii. refl.
-  Qed.
-  Next Obligation.
-  Proof.
-    ii. etrans; eauto.
-  Qed.
+End ValueMap.
 
 
-  Lemma le_le_partial m_tgt m_src (LE: le m_tgt m_src)
-    :
-      le_partial m_tgt m_src.
-  Proof.
-    ii. eapply SeqCell.le_le_partial. auto.
-  Qed.
+Module SeqMemory.
+  Record t :=
+    mk {
+        value_map: ValueMap.t;
+        flags: Flags.t;
+        deferred: Flags.t;
+      }.
 
-  Definition init (vals: Loc.t -> Const.t): t :=
-    fun loc => SeqCell.init (vals loc).
+  Definition read (loc: Loc.t) (m: t): Const.t :=
+    ValueMap.read loc m.(value_map).
 
-  Variant release: forall (m_before: t) (m_released: option t) (m_after: t), Prop :=
-  | release_some
-      m_before m_released m_after
-      (RELEASE: forall loc, SeqCell.release (m_before loc) (m_released loc) (m_after loc))
-    :
-      release m_before (Some m_released) m_after
-  | release_none
+  Definition write (loc: Loc.t) (v: Const.t) (m: t): t :=
+    mk (ValueMap.write loc v m.(value_map))
+       (Flags.update loc true m.(flags))
+       (Flags.update loc false m.(deferred)).
+
+  Variant acquire (cond: Loc.t -> bool) (v_acq: ValueMap.t):
+    forall (m_before: t) (f: Flags.t) (m_after: t), Prop :=
+  | acquire_intro
       m
+      (DEFERRED: Flags.is_empty m.(deferred))
     :
-      release m None m
+      acquire
+        cond
+        v_acq
+        m
+        (m.(flags))
+        (mk (ValueMap.acquire cond v_acq m.(value_map)) m.(flags) m.(deferred)).
+
+  Variant release:
+    forall (m_before: t) (f_rel: Flags.t) (v_rel: ValueMap.t) (m_after: t), Prop :=
+  | release_intro
+      d m
+      (DEFERRED: Flags.is_empty m.(deferred))
+    :
+      release
+        m
+        (Flags.join d m.(flags))
+        (ValueMap.release m.(value_map) d)
+        (mk m.(value_map) Flags.empty d)
+  .
+
+  Variant update:
+    forall
+      (loc: Loc.t) (v_new: Const.t)
+      (m_before: t)
+      (v: Const.t) (f: Flag.t)
+      (m_after: t), Prop :=
+  | update_intro
+      m loc v_new
+      (DEFERRED: m.(deferred) loc = false)
+    :
+      update
+        loc
+        v_new
+        m
+        (m.(value_map) loc)
+        (m.(flags) loc)
+        (mk (ValueMap.write loc v_new m.(value_map))
+            (Flags.update loc false m.(flags))
+            (m.(deferred)))
   .
 End SeqMemory.
+
+
+Module SeqEvent.
+  Record input :=
+    mk_input {
+        in_accessed: option (Loc.t * Const.t * Flag.t);
+        in_acquired: option (Flags.t);
+        in_released: option (ValueMap.t * Flags.t);
+      }.
+
+  Record output :=
+    mk_output {
+        out_accessed: option (Perm.t * Const.t);
+        out_acquired: option (Perms.t * ValueMap.t);
+        out_released: option (Perms.t);
+      }.
+
+  Definition wf_input (e: ProgramEvent.t) (i: input): Prop :=
+    (<<UPDATE: forall loc,
+        ((exists v_old f_old, i.(in_accessed) = Some (loc, v_old, f_old)) <-> is_accessing e = Some loc)>>) /\
+    (<<ACQUIRE: is_some i.(in_acquired) <-> is_acquire e>>) /\
+    (<<RELEASE: is_some i.(in_released) <-> is_release e>>)
+  .
+
+  Definition wf_output (e: ProgramEvent.t) (o: output): Prop :=
+    (<<UPDATE: is_some o.(out_accessed) <-> is_some (is_accessing e)>>) /\
+    (<<ACQUIRE: is_some o.(out_acquired) <-> is_acquire e>>) /\
+    (<<RELEASE: is_some o.(out_released) <-> is_release e>>)
+  .
+
+  Lemma wf_input_le e0 e1 i
+        (EVENT: ProgramEvent.le e0 e1)
+    :
+      wf_input e0 i <-> wf_input e1 i.
+  Proof.
+    unfold wf_input. destruct e0, e1; ss; des; clarify.
+  Qed.
+
+  Lemma wf_output_le e0 e1 o
+        (EVENT: ProgramEvent.le e0 e1)
+    :
+      wf_output e0 o <-> wf_output e1 o.
+  Proof.
+    unfold wf_output. destruct e0, e1; ss; des; clarify.
+  Qed.
+
+  Variant step_update:
+    forall (i: option (Loc.t * Const.t * Flag.t))(o: option (Perm.t * Const.t))
+           (p0: Perms.t) (m0: SeqMemory.t) (p1: Perms.t) (m1: SeqMemory.t), Prop :=
+  | step_update_none
+      p m
+    :
+      step_update
+        None None
+        p m p m
+  | step_update_some
+      loc v f p_new v_new
+      p0 m0 p1 m1
+      (PERM: p1 = Perms.update loc p_new p0)
+      (MEM: SeqMemory.update loc v_new m0 v f m1)
+    :
+      step_update
+        (Some (loc, v, f)) (Some (p_new, v_new))
+        p0 m0 p1 m1
+  .
+
+  Variant step_acquire:
+    forall (i: option (Flags.t)) (o: option (Perms.t * ValueMap.t))
+           (p0: Perms.t) (m0: SeqMemory.t) (p1: Perms.t) (m1: SeqMemory.t), Prop :=
+  | step_acquire_none
+      p m
+    :
+      step_acquire
+        None None
+        p m p m
+  | step_acquire_some
+      p_acq v_acq f
+      p0 m0 p1 m1
+      (PERM: p1 = Perms.join p0 p_acq)
+      (MEM: SeqMemory.acquire (Perms.acquired p0 p_acq) v_acq m0 f m1)
+    :
+      step_acquire
+        (Some f) (Some (p_acq, v_acq))
+        p0 m0 p1 m1
+  .
+
+  Variant step_release:
+    forall (i: option (ValueMap.t * Flags.t)) (o: option Perms.t)
+           (p0: Perms.t) (m0: SeqMemory.t) (p1: Perms.t) (m1: SeqMemory.t), Prop :=
+  | step_release_none
+      p m
+    :
+      step_release
+        None None
+        p m p m
+  | step_release_some
+      p_rel v_rel f_rel
+      p0 m0 p1 m1
+      (PERM: p1 = Perms.meet p0 p_rel)
+      (MEM: SeqMemory.release m0 f_rel v_rel m0)
+    :
+      step_release
+        (Some (v_rel, f_rel)) (Some p_rel)
+        p0 m0 p1 m1
+  .
+
+  Variant step:
+    forall (i: input) (o: output)
+           (p0: Perms.t) (m0: SeqMemory.t) (p1: Perms.t) (m1: SeqMemory.t), Prop :=
+  | step_intro
+      i o p0 m0 p1 m1 p2 m2 p3 m3
+      (UPD: step_update i.(in_accessed) o.(out_accessed) p0 m0 p1 m1)
+      (ACQ: step_acquire i.(in_acquired) o.(out_acquired) p1 m1 p2 m2)
+      (REL: step_release i.(in_released) o.(out_released) p2 m2 p3 m3)
+    :
+      step i o p0 m0 p3 m3
+  .
+End SeqEvent.
 
 
 Module SeqState.
@@ -273,7 +715,7 @@ Section LANG.
       m
       loc val ord
       (ORD: Ordering.le ord Ordering.na)
-      (VAL: Perm.le Perm.full (p loc) -> fst (m loc) = val)
+      (VAL: Perm.le Perm.high (p loc) -> Const.le val (SeqMemory.read loc m))
     :
       na_local_step
         p
@@ -284,7 +726,7 @@ Section LANG.
       loc val ord
       (ORD: Ordering.le ord Ordering.na)
       (MEM: SeqMemory.write loc val m0 = m1)
-      (PERM: e = if Perm.le Perm.full (p loc) then MachineEvent.silent else MachineEvent.failure)
+      (PERM: e = if Perm.le Perm.high (p loc) then MachineEvent.silent else MachineEvent.failure)
     :
       na_local_step
         p
@@ -332,137 +774,41 @@ End LANG.
 End SeqState.
 
 
-Variant diff :=
-| diff_none
-| diff_rel
-| diff_acq (v: Const.t)
-.
-
-Definition diffs := Loc.t -> diff.
-
-Definition update_mem
-           (d: diffs) (m0: SeqMemory.t): SeqMemory.t :=
-  fun loc =>
-    match (d loc) with
-    | diff_none | diff_rel => m0 loc
-    | diff_acq v1 => SeqCell.update v1 (m0 loc)
-    end.
-
-Definition update_perm (d: diffs) (p0: Perms.t): Perms.t :=
-  fun loc =>
-    match (d loc) with
-    | diff_none => p0 loc
-    | diff_acq _ => Perm.full
-    | diff_rel => Perm.none
-    end.
-
-
-Definition wf_diff_perms (l: option Loc.t) (d: diffs) (p: Perms.t): Prop :=
-  forall loc,
-    match (d loc), (p loc) with
-    | diff_none, _ => True
-    | diff_rel, Perm.full => True
-    | diff_acq _, Perm.none => True
-    | diff_acq _, Perm.full => l = Some loc
-    | _, _ => False
-    end.
-
-Definition wf_diff_event (d: diffs) (e: ProgramEvent.t): Prop :=
-  match e with
-  | ProgramEvent.syscall _ => True
-  | ProgramEvent.read loc val ord =>
-    forall loc' (NEQ: loc' <> loc),
-      match (d loc') with
-      | diff_rel => False
-      | diff_acq _ => Ordering.le Ordering.acqrel ord
-      | diff_none => True
-      end
-  | ProgramEvent.write loc _ ord =>
-    forall loc' (NEQ: loc' <> loc),
-      match (d loc') with
-      | diff_acq _ => False
-      | diff_rel => Ordering.le Ordering.strong_relaxed ord
-      | diff_none => True
-      end
-  | ProgramEvent.update loc _ _ ordr ordw =>
-    forall loc' (NEQ: loc' <> loc),
-      match (d loc') with
-      | diff_rel => Ordering.le Ordering.strong_relaxed ordw
-      | diff_acq _ => Ordering.le Ordering.acqrel ordr
-      | diff_none => True
-      end
-  | ProgramEvent.fence ordr ordw =>
-    forall loc',
-      match (d loc') with
-      | diff_rel => Ordering.le Ordering.strong_relaxed ordw
-      | diff_acq _ => Ordering.le Ordering.acqrel ordr
-      | diff_none => True
-      end
-  | _ => True
-  end.
-
-Definition wf_released (m_released: option SeqMemory.t) (e: ProgramEvent.t): Prop :=
-  match m_released with
-  | Some _ => is_release_event e
-  | None => ~ is_release_event e
-  end.
-
-Definition match_cell (l: option Loc.t) (c: option SeqCell.t) (m: SeqMemory.t): Prop :=
-  match l, c with
-  | Some l, Some c => SeqCell.le c (m l)
-  | None, None => True
-  | _, _ => False
-  end.
-
-Definition update_cell (l: option Loc.t) (c: option SeqCell.t) (m: SeqMemory.t): SeqMemory.t :=
-  match l, c with
-  | Some l, Some c => SeqMemory.update l c m
-  | _, _ => m
-  end.
-
-Definition wf_cell (c: option SeqCell.t) (e: ProgramEvent.t): Prop :=
-  match (is_accessing e) with
-  | Some loc => is_some c
-  | _ => ~ is_some c
-  end.
-
-
 Module Oracle.
-  Definition t: Type. Admitted.
+  Record t :=
+    mk {
+        _t: Type;
+        _step: ProgramEvent.t -> SeqEvent.input -> SeqEvent.output -> _t -> _t -> Prop;
+        _o: _t;
+      }.
 
-  Definition step:
-    forall (p0: Perms.t)
-           (e: ProgramEvent.t)
-           (c0: option SeqCell.t)
-           (d: diffs)
-           (m_released: option SeqMemory.t)
-           (o0: t)
-           (o1: t), Prop.
-  Admitted.
+  Variant step: forall (pe: ProgramEvent.t) (i: SeqEvent.input) (o: SeqEvent.output) (o0 o1: t), Prop :=
+  | step_intro
+      pe i o
+      _t (_step: ProgramEvent.t -> SeqEvent.input -> SeqEvent.output -> _t -> _t -> Prop)
+      (x0 x1: _t)
+      (STEP: _step pe i o x0 x1)
+    :
+      step pe i o (@mk _t _step x0) (@mk _t _step x1)
+  .
 
-  Definition progress e o0 p0 c0 d: Prop :=
-    forall m_released (WF: wf_released m_released e),
-      exists o1, step p0 e c0 d m_released o0 o1.
+  Definition progress pe o0: Prop :=
+    forall i (WF: SeqEvent.wf_input pe i),
+    exists o o1, (<<STEP: step pe i o o0 o1>>) /\ (<<WF: SeqEvent.wf_output pe o>>).
 
   Variant _wf (wf: t -> Prop): t -> Prop :=
   | wf_intro
       (o0: t)
-      (WF: forall p0 e c0 d (m_released: option SeqMemory.t) (o1: t)
-                  (STEP: step p0 e c0 d m_released o0 o1),
-          (<<EVENT: wf_diff_event d e>>) /\
-          (<<PERM: wf_diff_perms (is_accessing e) d p0>>) /\
-          (<<CELL: wf_cell c0 e>>) /\
-          (<<RELEASED: wf_released m_released e>>) /\
+      (WF: forall pe i o o1 (STEP: step pe i o o0 o1),
+          (<<INPUT: SeqEvent.wf_input pe i>>) /\
+          (<<OUTPUT: SeqEvent.wf_output pe o>>) /\
           (<<ORACLE: wf o1>>))
-      (LOAD: forall p0 c0 loc ord
-                    (ORD: Ordering.le ord Ordering.strong_relaxed),
-          exists v d, progress (ProgramEvent.read loc v ord) o0 p0 (Some c0) d)
-      (STORE: forall p0 c0 loc ord val,
-          exists d, progress (ProgramEvent.write loc val ord) o0 p0 c0 d)
-      (FENCE: forall p0 ordr ordw
-                     (ORDR: Ordering.le ordr Ordering.strong_relaxed)
-                     (ORDW: Ordering.le ordw Ordering.acqrel),
-          exists d, progress (ProgramEvent.fence ordr ordw) o0 p0 None d)
+      (LOAD: forall loc ord,
+          exists val, progress (ProgramEvent.read loc val ord) o0)
+      (STORE: forall loc ord val,
+          progress (ProgramEvent.write loc val ord) o0)
+      (FENCE: forall ordr ordw,
+          progress (ProgramEvent.fence ordr ordw) o0)
     :
       _wf wf o0
   .
@@ -509,31 +855,40 @@ Section LANG.
   Qed.
 
   Variant at_step:
-    forall (e: ProgramEvent.t) (d: diffs) (m_released: option SeqMemory.t)
+    forall (e: ProgramEvent.t) (i: SeqEvent.input) (o: SeqEvent.output)
            (th0: t) (th1: t), Prop :=
   | at_step_intro
-      p0 p1 o0 o1 e c d m_released st0 st1 m0 m_upd m1
-      (STEP: lang.(Language.step) e st0 st1)
-      (ORACLE: Oracle.step p0 e c d m_released o0 o1)
-      (CELL: match_cell (is_accessing e) c m0)
-      (PERM: p1 = update_perm d p0)
-      (MEM: m_upd = update_mem d (update_cell (is_accessing e) c m0))
-      (RELEASE: SeqMemory.release m_upd m_released m1)
+      e0 e1 i o
+      st0 st1 p0 p1 o0 o1 m0 m1
+      (LANG: lang.(Language.step) e1 st0 st1)
+      (EVENT: ProgramEvent.le e0 e1)
+      (ORACLE: Oracle.step e0 i o o0 o1)
+      (MEM: SeqEvent.step i o p0 m0 p1 m1)
     :
-      at_step e d m_released (mk (SeqState.mk _ st0 m0) p0 o0) (mk (SeqState.mk _ st1 m1) p1 o1)
+      at_step e0 i o (mk (SeqState.mk _ st0 m0) p0 o0) (mk (SeqState.mk _ st1 m1) p1 o1)
   .
 
   Variant step (e: MachineEvent.t) (th0: t) (th1: t): Prop :=
   | step_na_step
       (STEP: na_step e th0 th1)
   | step_at_step
-      pe d m_released
+      pe i o
       (EVENT: e = get_machine_event pe)
-      (STEP: at_step pe d m_released th0 th1)
+      (STEP: at_step pe i o th0 th1)
   .
 
   Definition failure (th0: t): Prop :=
     exists th1, (<<FAILURE: step MachineEvent.failure th0 th1>>).
+
+  Variant non_acquire_step (e: MachineEvent.t) (th0: t) (th1: t): Prop :=
+  | non_acquire_step_na_step
+      (STEP: na_step e th0 th1)
+  | non_acquire_step_at_step
+      pe i o
+      (ACQUIRE: ~ is_acquire pe)
+      (EVENT: e = get_machine_event pe)
+      (STEP: at_step pe i o th0 th1)
+  .
 End LANG.
 End SeqThread.
 
@@ -553,7 +908,10 @@ Section SIMULATION.
       (<<STEPS: rtc (SeqState.na_step p0 MachineEvent.silent) st_src0 st_src1>>) /\
       (<<TERMINAL_SRC: lang_src.(Language.is_terminal) st_src1.(SeqState.state)>>) /\
       (<<TERMINAL: sim_terminal st_src1.(SeqState.state) st_tgt0.(SeqState.state)>>) /\
-      (<<MEM: SeqMemory.le st_tgt0.(SeqState.memory) st_src1.(SeqState.memory)>>).
+      (<<VALUE: ValueMap.le st_tgt0.(SeqState.memory).(SeqMemory.value_map) st_tgt0.(SeqState.memory).(SeqMemory.value_map)>>) /\
+      (<<FLAG: Flags.le st_tgt0.(SeqState.memory).(SeqMemory.flags) st_tgt0.(SeqState.memory).(SeqMemory.flags)>>) /\
+      (<<DEFERRED: Flags.is_empty st_tgt0.(SeqState.memory).(SeqMemory.deferred) -> Flags.is_empty st_src0.(SeqState.memory).(SeqMemory.deferred)>>)
+  .
 
   Definition sim_seq_na_step_case
              (sim_seq:
@@ -579,24 +937,20 @@ Section SIMULATION.
              (p0: Perms.t)
              (st_src0: SeqState.t lang_src)
              (st_tgt0: SeqState.t lang_tgt): Prop :=
-    forall st_tgt1 e
-           (STEP_TGT: lang_tgt.(Language.step) e st_tgt0.(SeqState.state) st_tgt1)
-           (ATOMIC: is_atomic_event e),
-    exists st_src1 st_src2,
+    forall st_tgt1 e_tgt
+           (STEP_TGT: lang_tgt.(Language.step) e_tgt st_tgt0.(SeqState.state) st_tgt1)
+           (ATOMIC: is_atomic_event e_tgt),
+    exists st_src1 st_src2 e_src,
       (<<STEPS: rtc (SeqState.na_step p0 MachineEvent.silent) st_src0 st_src1>>) /\
-      (<<MEM: is_acquire_event e -> SeqMemory.le_partial st_tgt0.(SeqState.memory) st_src1.(SeqState.memory)>>) /\
-      (<<STEP: lang_src.(Language.step) e st_src1.(SeqState.state) st_src2>>) /\
-      (<<SIM: forall d c mem_released mem_tgt
-                     (EVENT: wf_diff_event d e)
-                     (PERM: wf_diff_perms (is_accessing e) d p0)
-                     (RELEASED: wf_released mem_released e)
-                     (CELL: wf_cell c e)
-                     (MATCH: match_cell (is_accessing e) c st_tgt0.(SeqState.memory))
-                     (MEM: SeqMemory.release (update_mem d (update_cell (is_accessing e) c st_tgt0.(SeqState.memory))) mem_released mem_tgt),
+      (<<STEP: lang_src.(Language.step) e_src st_src1.(SeqState.state) st_src2>>) /\
+      (<<EVENT: ProgramEvent.le e_src e_tgt>>) /\
+      (<<SIM: forall i o p1 mem_tgt
+                     (INPUT: SeqEvent.wf_input e_tgt i)
+                     (OUTPUT: SeqEvent.wf_output e_tgt o)
+                     (STEP_TGT: SeqEvent.step i o p0 st_tgt0.(SeqState.memory) p1 mem_tgt),
           exists mem_src,
-            (<<MATCH: match_cell (is_accessing e) c st_src1.(SeqState.memory)>>) /\
-            (<<MEM: SeqMemory.release (update_mem d (update_cell (is_accessing e) c st_src1.(SeqState.memory))) mem_released mem_src>>) /\
-            (<<SIM: sim_seq (update_perm d p0)
+            (<<STEP_SRC: SeqEvent.step i o p0 st_src1.(SeqState.memory) p1 mem_src>>) /\
+            (<<SIM: sim_seq p1
                             (SeqState.mk _ st_src2 mem_src)
                             (SeqState.mk _ st_tgt1 mem_tgt)>>)>>).
 
@@ -604,17 +958,20 @@ Section SIMULATION.
              (p0: Perms.t)
              (st_src0: SeqState.t lang_src)
              (st_tgt0: SeqState.t lang_tgt): Prop :=
-    forall o (WF: Oracle.wf o),
+    forall o (WF: Oracle.wf o)
+           (DEFERRED: Flags.is_empty st_tgt0.(SeqState.memory).(SeqMemory.deferred)),
     exists th,
-      (<<STEPS: rtc (SeqThread.step MachineEvent.silent) (SeqThread.mk st_src0 p0 o) th>>) /\
-      ((<<MEM: SeqMemory.le_partial st_tgt0.(SeqState.memory) th.(SeqThread.state).(SeqState.memory)>>) \/ (<<FAILURE: SeqThread.failure th>>)).
+      (<<STEPS: rtc (SeqThread.non_acquire_step MachineEvent.silent) (SeqThread.mk st_src0 p0 o) th>>) /\
+      ((<<FLAG: Flags.le st_tgt0.(SeqState.memory).(SeqMemory.flags) th.(SeqThread.state).(SeqState.memory).(SeqMemory.flags)>>) /\
+       (<<DEFERRED: Flags.is_empty th.(SeqThread.state).(SeqState.memory).(SeqMemory.deferred)>>)
+       \/ (<<FAILURE: SeqThread.failure th>>)).
 
   Definition sim_seq_failure_case
              (p0: Perms.t)
              (st_src0: SeqState.t lang_src): Prop :=
     forall o (WF: Oracle.wf o),
     exists th,
-      (<<STEPS: rtc (SeqThread.step MachineEvent.silent) (SeqThread.mk st_src0 p0 o) th>>) /\
+      (<<STEPS: rtc (SeqThread.non_acquire_step MachineEvent.silent) (SeqThread.mk st_src0 p0 o) th>>) /\
       (<<FAILURE: SeqThread.failure th>>).
 
 
@@ -652,11 +1009,12 @@ Section SIMULATION.
 
 
   Lemma sim_seq_partial_imm p st_src st_tgt
-        (MEM: SeqMemory.le_partial st_tgt.(SeqState.memory) st_src.(SeqState.memory))
+        (FLAGS: Flags.le st_tgt.(SeqState.memory).(SeqMemory.flags) st_src.(SeqState.memory).(SeqMemory.flags))
+        (DEFERRED: Flags.is_empty st_tgt.(SeqState.memory).(SeqMemory.deferred) -> Flags.is_empty st_src.(SeqState.memory).(SeqMemory.deferred))
     :
       sim_seq_partial_case p st_src st_tgt.
   Proof.
-    ii. esplits; [refl|]. left. auto.
+    ii. esplits; [refl|]. left. splits; auto.
   Qed.
 
   Lemma sim_seq_failure_imm p0 st_src0 st_tgt0 st_src1
@@ -669,11 +1027,11 @@ Section SIMULATION.
   Qed.
 
   Definition sim_seq_all (st_src: lang_src.(Language.state)) (st_tgt: lang_tgt.(Language.state)): Prop :=
-    forall p vals,
+    forall p m,
       sim_seq
         p
-        (SeqState.mk _ st_src (SeqMemory.init vals))
-        (SeqState.mk _ st_tgt (SeqMemory.init vals)).
+        (SeqState.mk _ st_src m)
+        (SeqState.mk _ st_tgt m).
 End SIMULATION.
 Arguments sim_seq [_] [_] _ _ _.
 #[export] Hint Resolve sim_seq_mon: paco.
